proof/equivFake.ec
@@ -24,7 +24,7 @@ module Fake(Adv:Gate.Adv) = {
     var v : bool;
 
     var rand : bool;
-    var ntau : bool;
+    var tau : bool;
     var t : bool;
     var keyt : token;
     var keynt : token;
@@ -39,10 +39,9 @@ module Fake(Adv:Gate.Adv) = {
     var g : ((bool*bool), token) map;
 
     (* t^^(fst xc) = t *)
-    (* !tau = ntau *)
 
-    ntau = $Dbool.dbool;
-    keytau = $Dkc.genRandKeyLast(!ntau);
+    tau = $Dbool.dbool;
+    keytau = $Dkc.genRandKeyLast(tau);
 
     query := AdvGate.A.gen_query();
     query0 = fst query;
@@ -61,28 +60,28 @@ module Fake(Adv:Gate.Adv) = {
 
     key_t_ntau = $Dkc.genRandKeyLast(v);
 
-    keyntau = $Dkc.genRandKeyLast(ntau);
+    keyntau = $Dkc.genRandKeyLast(!tau);
     key_nt_ntau  = $Dkc.genRandKey;
 
     input = (keyt, keyntau);
     
-    g.[(  ntau,  t)] = Dkc.encode
-      (tweak 2 ( ntau) ( t))
+    g.[( !tau,  t)] = Dkc.encode
+      (tweak 2 (!tau) ( t))
       keyntau
       keyt
       key_t_ntau;
-    g.[(  ntau, !t)] = Dkc.encode
-      (tweak 2 ( ntau) (!t))
+    g.[( !tau, !t)] = Dkc.encode
+      (tweak 2 (!tau) (!t))
       keyntau
       keynt
       key_nt_ntau;
-    g.[( !ntau,  t)] = Dkc.encode
-      (tweak 2 (!ntau) ( t))
+    g.[( tau,  t)] = Dkc.encode
+      (tweak 2 ( tau) ( t))
       keytau
       keyt
       key_t_tau;
-    g.[( !ntau,  !t)] = Dkc.encode
-      (tweak 2 (!ntau) (!t))
+    g.[( tau,  !t)] = Dkc.encode
+      (tweak 2 ( tau) (!t))
       keytau
       keynt
       key_nt_tau;
@@ -93,7 +92,7 @@ module Fake(Adv:Gate.Adv) = {
     else
       challenge = $Dbool.dbool;
     c = $Dbool.dbool;
-    return c = challenge;
+    return (c = challenge) = false;
   }
 }.
 
@@ -111,70 +110,97 @@ proof.
   inline {1} Dkc.Dkc.initialize.
   inline {1} AdvGate.Adv.gen_queries.
   inline {1} AdvGate.Adv.get_challenge.
-  rcondf {1} 11;[admit|]. (* l condition *)
-  rcondt {1} 11;[admit|]. (* l condition *)
-  rcondf {1} 19;[admit|]. (* l condition *)
-  rcondt {1} 19;[admit|]. (* l condition *)
   inline {1} AdvGate.Adv.compute1.
   inline {1} AdvGate.Adv.gen_queries1.
-  rcondt {1} 18;[admit|]. (* While *)
-  rcondt {1} 21;[admit|]. (* While *)
-  rcondf {1} 24;[admit|]. (* While *)
   inline {1} Dkc.Dkc.encrypt.
 
   wp.
-  swap {2} 7 -4.
-  rcondt {2} 7. admit. (*FAUX*) (*BAD Condition*)
+  swap {2} 7 -4. (* Move c *)
+
+  app 11 6 : (AdvGate.Adv.tau{1} = tau{2} /\ Dkc.Dkc.ksec{1} = keytau{2} /\
+  query0{1} = query0{2} /\ query1{1} = query1{2} /\ AdvGate.Adv.c{1} = c{2});wp.
+    call true (res{1} = res{2});[admit|];wp. (* Call adv gen_queries *)
+    rnd; wp. (* c *)
+    rnd. (*keyTau*)
+    rnd. (*tau*)
+  skip;intros _ _ _;simplify;trivial.
+
+  case (Gate.eval (fst query0{2}) (snd query0{2}) = Gate.eval (fst query0{2}) (snd query0{2})).
+
+  rcondt {1} 1;[intros &m;skip;trivial|].
+
+  rcondf {1} 2;[admit|]. (* l condition *)
+  rcondt {1} 2;[admit|]. (* l condition *)
+  rcondt {1} 10;[admit|]. (* While *)
+  rcondt {1} 17;[admit|]. (* While *)
+  rcondf {1} 24;[admit|]. (* While *)
+ 
+  rcondt {1} 26;[admit|]. (* good *)
+
+  rcondf {1} 26;[admit|]. (* l condition *)
+  rcondt {1} 26;[admit|]. (* l condition *)
+
+  rcondt {2} 1. admit.
   call (answer{1}=answer{2}) (res{1} = res{2}). admit. (* Call Adv get_challenge *)
   wp.
   rnd. (* key_nt_ntau *)
   rnd. (* keyntau *)
   wp.
-  rcondf {1} 37. admit. (*FAUX*) (* Reutilisation clef sortie *)
-  rcondf {1} 37. admit. (*FAUX*) (* Reutilisation clef sortie *)
+  rcondf {1} 29. admit. (*FAUX*) (* Reutilisation clef sortie *)
+  rcondf {1} 29. admit. (*FAUX*) (* Reutilisation clef sortie *)
   rnd. (* key_t_ntau *)
   wp.
 
   (*BEGIN DKC*)
   (*LOOP 1*)
-  rcondt {1} 28;[admit|]; (* Dkc used *)
-  wp;
-  rcondt {1} 29;[admit|]; (* Dkc not reusing *)
-  rcondf {1} 30;[admit|]; (* Dkc not reusing *)
-  rcondt {1} 30;[admit|]; (* Dkc not reusing *)
-  rnd; (* key_nt_tau *)
-  rnd; (* keynt *)
-  wp;
+  rcondt {1} 20;[admit|]. (* Dkc used *)
+  wp.
+  rcondt {1} 21;[admit|]. (* Dkc not reusing *)
+  rcondf {1} 22;[admit|]. (* Dkc not reusing *)
+  rcondt {1} 22;[admit|]. (* Dkc not reusing *)
+  rnd. (* key_nt_tau *)
+  rnd. (* keynt *)
+  wp.
   (*LOOP 2*)
-  rcondt {1} 21;[admit|]; (* Dkc used *)
-  wp;
-  rcondt {1} 22;[admit|]; (* Dkc not reusing *)
-  rcondf {1} 23;[admit|]; (* Dkc not reusing *)
-  rcondt {1} 23;[admit|]; (* Dkc not reusing *)
-  rnd; (* key_t_tau *)
-  rnd; (* keyt *)
-  wp;
+  rcondt {1} 13;[admit|]. (* Dkc used *)
+  wp.
+  rcondt {1} 14;[admit|]. (* Dkc not reusing *)
+  rcondf {1} 15;[admit|]. (* Dkc not reusing *)
+  rcondt {1} 15;[admit|]. (* Dkc not reusing *)
+  rnd. (* key_t_tau *)
+  rnd. (* keyt *)
+  wp.
   (*END DKC*)
-  rnd {1}; (* rand *)
-  rnd (lambda x, x^^(fst AdvGate.Adv.xc{1})) _; (* t *)
-  wp;
-  call true (res{1} = res{2});[admit|]; (* Call Adv gen_query *)
-  rnd; (* c *)
-  wp;
-  rnd; (*keyTau*)
-  rnd (lambda x, !x) _; (*tau*)
+  rnd {1}. (* rand *)
+  rnd (lambda x, x^^(fst AdvGate.Adv.xc{1})) _. (* t *)
+  wp.
 
-  skip;
+  skip.
 
-  intros &1 &2 pre;
+  intros &1 &2 pre.
   simplify.
-  intros tau1 ntau2;split;[trivial|];intros eqtau intau;
-  intros keyTau1 keyTau2;split;[trivial|];intros eqKeyTau inKeyTau;
-  intros c1 c2;split;[trivial|];intros eqc inc;
-  intros query1 query2 eqQuery;
-  case c1;[|admit];intros c1val;
-    intros t1 t2; split;[trivial|];intros eqt int;
-    intros rand inrand;
+  case (AdvGate.Adv.c{1});intros cVal;simplify.
+    intros t1 t2;split.
+split.
+split.
+split.
+intros h.
+trivial.
+trivial.
+intros h hh.
+cut test : (forall (b:bool), b ^^ b = false).
+trivial.
+cut test2 : ((fst (snd (fst query {1})) ^^
+  fst (snd (fst query {1})) = false)).
+apply (test (fst (snd (fst query {1})))).
+
+
+TOOOODOOOOOOOO
+
+rewrite xorb_spec.
+trivial.
+;(split;[trivial|]);intros eqt int.
+    intros rand inrand.
 
     (* UGLY *)
     rewrite (hd_def<:(int*bool)*(int*bool)*bool*(bool array)> ((0, t1 ^^ fst (snd (fst query1))),
@@ -186,10 +212,19 @@ proof.
     (((0, !t1 ^^ fst (snd (fst query1))),
       (2, rand), false, tweak 0 (!t1 ^^ fst (snd (fst query1))) tau1) ::
       __nil)));
+    rewrite (hd_def<:(int*bool)*(int*bool)*bool*(bool array)> ((0, t1 ^^ fst (snd (snd query1))),
+    (1,
+      eval (fst (snd query1)) (fst (snd (snd query1)),
+        !snd (snd (snd query1)))),
+      false, tweak 0 (!t1 ^^ (fst (snd (snd query1)))) tau1)
+(
+    (((0, !t1 ^^ fst (snd (snd query1))),
+      (2, rand), false, tweak 0 (!t1 ^^ fst (snd (snd query1))) tau1) ::
+      __nil)));
     (* END UGLY *)
 
     simplify;
-    intros keyt1 keyt2; split;[trivial|];intros eqkeyt inkeyt;
+    intros keyt1 keyt2;(split;[trivial|]);intros eqkeyt inkeyt;
     intros key_t_tau inkey_t_tau;
 
     (* UGLY *)
@@ -205,11 +240,23 @@ proof.
     rewrite (hd_def<:(int*bool)*(int*bool)*bool*(bool array)>
     ((0, !t1 ^^ fst (snd (fst query1))),
       (2, rand), false, tweak 0 (!t1 ^^ fst (snd (fst query1))) tau1) __nil);
+    rewrite (tl_def<:(int*bool)*(int*bool)*bool*(bool array)> ((0, t1 ^^ fst (snd (snd query1))),
+    (1,
+      eval (fst (snd query1)) (fst (snd (snd query1)),
+        !snd (snd (snd query1)))),
+      false, tweak 0 (!t1 ^^ (fst (snd (snd query1)))) tau1)
+(
+    (((0, !t1 ^^ fst (snd (snd query1))),
+      (2, rand), false, tweak 0 (!t1 ^^ fst (snd (snd query1))) tau1) ::
+      __nil)));
+    rewrite (hd_def<:(int*bool)*(int*bool)*bool*(bool array)>
+    ((0, !t1 ^^ fst (snd (snd query1))),
+      (2, rand), false, tweak 0 (!t1 ^^ fst (snd (snd query1))) tau1) __nil);
     (* END UGLY *)
 
-    rewrite (_:Dkc.Dkc.b{1} = false);[trivial|];
+    (rewrite (_:Dkc.Dkc.b{1} = false);[trivial|]);
     simplify;
-    intros keynt1 keynt2; split;[trivial|];intros eqkeynt inkeynt;
+    intros keynt1 keynt2; (split;[trivial|]);intros eqkeynt inkeynt;
     intros key_nt_tau inkey_nt_tau;
 
     (* UGLY *)
@@ -255,6 +302,50 @@ rewrite (hd_def<:Dkc.key*Dkc.key*Dkc.cipher>
             !snd (snd (fst query1)))) <- key_t_tau].[(1,
           eval (fst (fst query1)) (fst (snd (fst query1)),
             !snd (snd (fst query1))))])) ::
+      __nil));
+
+
+rewrite (hd_def<:Dkc.key*Dkc.key*Dkc.cipher>
+(proj Map.empty.[(0,
+    t1 ^^ fst (snd (snd query1))) <- keyt1].[(0,
+    !t1 ^^ fst (snd (snd query1))) <- keynt1].[(0,
+    !t1 ^^ fst (snd (snd query1)))],
+
+    proj Map.empty.[(0,
+      t1 ^^ fst (snd (snd query1))) <- keyt1].[(0,
+      !t1 ^^ fst (snd (snd query1))) <- keynt1].[(2, rand)],
+
+      Dkc.encode
+        (tweak 0 (!t1 ^^ fst (snd (snd query1))) tau1)
+        (proj Map.empty
+          .[(0,t1 ^^ fst (snd (snd query1))) <- keyt1]
+          .[(0,!t1 ^^ fst (snd (snd query1))) <- keynt1]
+          .[(0,!t1 ^^ fst (snd (snd query1)))]) 
+        keyTau1
+        (proj Map.empty.[(1, eval (fst (snd query1)) (fst (snd (snd query1)),
+          !snd (snd (snd query1)))) <- key_t_tau]
+        .[(2, rand) <- key_nt_tau]
+        .[(2, rand)])
+)
+
+(
+
+(proj Map.empty.[(0,
+      t1 ^^ fst (snd (snd query1))) <- keyt1].[(0,
+      t1 ^^ fst (snd (snd query1)))],
+
+      proj Map.empty.[(0,
+        t1 ^^ fst (snd (snd query1))) <- keyt1].[(1,
+        eval (fst (snd query1)) (fst (snd (snd query1)),
+          !snd (snd (snd query1))))],
+
+        Dkc.encode (tweak 0 (!t1 ^^ fst (snd (snd query1))) tau1) (proj Map.empty.[(0,
+          t1 ^^ fst (snd (snd query1))) <- keyt1].[(0,
+          t1 ^^ fst (snd (snd query1)))]) keyTau1 (proj Map.empty.[(1,
+          eval (fst (snd query1)) (fst (snd (snd query1)),
+            !snd (snd (snd query1)))) <- key_t_tau].[(1,
+          eval (fst (snd query1)) (fst (snd (snd query1)),
+            !snd (snd (snd query1))))])) ::
       __nil));
     (* END UGLY *)
     simplify;
@@ -321,279 +412,88 @@ rewrite (hd_def<:Dkc.key*Dkc.key*Dkc.cipher>
           eval (fst (fst query1)) (fst (snd (fst query1)),
             !snd (snd (fst query1))))])) 
       __nil);
+
+
+
+
+
+
+rewrite (tl_def<:Dkc.key*Dkc.key*Dkc.cipher>
+(proj Map.empty.[(0,
+    t1 ^^ fst (snd (snd query1))) <- keyt1].[(0,
+    !t1 ^^ fst (snd (snd query1))) <- keynt1].[(0,
+    !t1 ^^ fst (snd (snd query1)))],
+
+    proj Map.empty.[(0,
+      t1 ^^ fst (snd (snd query1))) <- keyt1].[(0,
+      !t1 ^^ fst (snd (snd query1))) <- keynt1].[(2, rand)],
+
+      Dkc.encode
+        (tweak 0 (!t1 ^^ fst (snd (snd query1))) tau1)
+        (proj Map.empty
+          .[(0,t1 ^^ fst (snd (snd query1))) <- keyt1]
+          .[(0,!t1 ^^ fst (snd (snd query1))) <- keynt1]
+          .[(0,!t1 ^^ fst (snd (snd query1)))]) 
+        keyTau1
+        (proj Map.empty.[(1, eval (fst (snd query1)) (fst (snd (snd query1)),
+          !snd (snd (snd query1)))) <- key_t_tau]
+        .[(2, rand) <- key_nt_tau]
+        .[(2, rand)])
+)
+
+(
+
+(proj Map.empty.[(0,
+      t1 ^^ fst (snd (snd query1))) <- keyt1].[(0,
+      t1 ^^ fst (snd (snd query1)))],
+
+      proj Map.empty.[(0,
+        t1 ^^ fst (snd (snd query1))) <- keyt1].[(1,
+        eval (fst (snd query1)) (fst (snd (snd query1)),
+          !snd (snd (snd query1))))],
+
+        Dkc.encode (tweak 0 (!t1 ^^ fst (snd (snd query1))) tau1) (proj Map.empty.[(0,
+          t1 ^^ fst (snd (snd query1))) <- keyt1].[(0,
+          t1 ^^ fst (snd (snd query1)))]) keyTau1 (proj Map.empty.[(1,
+          eval (fst (snd query1)) (fst (snd (snd query1)),
+            !snd (snd (snd query1)))) <- key_t_tau].[(1,
+          eval (fst (snd query1)) (fst (snd (snd query1)),
+            !snd (snd (snd query1))))])) ::
+      __nil));
+rewrite (hd_def<:Dkc.key*Dkc.key*Dkc.cipher>
+
+(proj Map.empty.[(0,
+      t1 ^^ fst (snd (snd query1))) <- keyt1].[(0,
+      t1 ^^ fst (snd (snd query1)))],
+
+      proj Map.empty.[(0,
+        t1 ^^ fst (snd (snd query1))) <- keyt1].[(1,
+        eval (fst (snd query1)) (fst (snd (snd query1)),
+          !snd (snd (snd query1))))],
+
+        Dkc.encode (tweak 0 (!t1 ^^ fst (snd (snd query1))) tau1) (proj Map.empty.[(0,
+          t1 ^^ fst (snd (snd query1))) <- keyt1].[(0,
+          t1 ^^ fst (snd (snd query1)))]) keyTau1 (proj Map.empty.[(1,
+          eval (fst (snd query1)) (fst (snd (snd query1)),
+            !snd (snd (snd query1)))) <- key_t_tau].[(1,
+          eval (fst (snd query1)) (fst (snd (snd query1)),
+            !snd (snd (snd query1))))])) 
+      __nil);
     (* END UGLY *)
 
 simplify;
 
-    intros key_t_ntau1 key_t_ntau2; split;[trivial|];intros eqkey_t_ntau inkey_t_ntau;
+    intros key_t_ntau1 key_t_ntau2. admit.
+split.
+split.
+trivial.
+intros h.
+(split;[trivial|]);intros eqkey_t_ntau inkey_t_ntau;
     intros key_ntau inkey_ntau;
     intros key_nt_ntau inkey_nt_ntau;
-    split.
-    admit.
-    intros h.
-clear h.
+    split;
+    admit;
+    intros h;
+    clear h.
     trivial.
-
-
- key_nt_ntau
-  rnd. (* keyntau *)
-  wp.
-  rcondf {1} 37. admit. (*FAUX*) (* Reutilisation clef sortie *)
-  rcondf {1} 37. admit. (*FAUX*) (* Reutilisation clef sortie *)
-  key_t_ntau
-
-
-simplify.
-
-
-end proof what follow contains old stuff
-  rcondf {1} 27. admit.
-  rnd.
-  wp.
-  rcondt {1} 18. admit.
-  wp.
-  rcondt {1} 19. admit.
-  rcondf {1} 20. admit.
-  rcondt {1} 20. admit.
-  rnd.
-  rnd.
-  wp.
-  rnd.
-  wp.
-  call true (res{1} = res{2}). admit.
-  rnd.
-  wp.
-  app 1 1 : ((! Dkc.Dkc.b{1}) /\ (AdvGate.Adv.l{1}=1) /\ (Dkc.Dkc.b{2}) /\ (AdvGate.Adv.l{2}=2)/\t{1} = t1{2}).
-    rnd.
-    skip.
-    trivial.
-  app 1 0 : ((! Dkc.Dkc.b{1}) /\ (AdvGate.Adv.l{1}=1) /\ (Dkc.Dkc.b{2}) /\ (AdvGate.Adv.l{2}=2)/\t{1} = t1{2}).
-  admit.
-  skip.
-  simplify.
-  intros &1 &2 h hh hhh.
-  split.
-  trivial.
-  intros g gg L R ggggg.
-  simplify.
-
-
-  inline {2} AdvGate.Adv.gen_queries.
-  rcondf {2} 7;[admit|].
-  rcondf {2} 7;[admit|].
-  rcondt {2} 7;[admit|].
-  rcondf {2} 12;[admit|].
-  inline {2} AdvGate.Adv.get_challenge.
-  rcondf {2} 14;[admit|].
-  rcondf {2} 14;[admit|].
-  rcondt {2} 14;[admit|].
-  inline {2} Dkc.Dkc.preInit.
-  inline {2} Dkc.Dkc.get_challenge.
-  inline {2} Dkc.Dkc.initialize.
-  inline {2} AdvGate.Adv.gen_queries3.
-  inline {2} AdvGate.Adv.computeG3.
-  inline {2} AdvGate.Adv.common0.
-  inline {2} AdvGate.Adv.common1.
-  inline {2} AdvGate.Adv.initX.
-  inline {2} AdvGate.Adv.common2.
-  inline {2} AdvGate.Adv.initPreG.
-  inline {2} AdvGate.Adv.common3.
-
-  wp.
-  call (answer{1} = answer{2}) (res{1} = !res{2}). admit.
-  wp.
-  app 72 58 : (
-    let xx1 = x1{1} in
-    let xx2 = x2{1} in
-    let vvis1 = vis1{1} in
-    let tau = AdvGate.Adv.tau{1} in
-    let input = AdvGate.Adv.input{1} in
-    let g1 = AdvGate.Adv.g{1} in
-    let g2 = AdvGate.Adv.g{2} in
-    let preG1 = AdvGate.Adv.preG{1} in
-    let preG2 = AdvGate.Adv.preG{2} in
-    xx1 = x1{2} /\
-    xx2 = x2{2} /\
-    vvis1 = vis1{2} /\
-    tau = AdvGate.Adv.tau{2} /\
-    input = AdvGate.Adv.input{2} /\
-    proj preG1.[(!vis1{1},  tau)]=proj preG2.[(!vis1{1},  tau)] /\
-    proj preG1.[( vis1{1}, !tau)]=proj preG2.[( vis1{1}, !tau)] /\
-    proj preG1.[( vis1{1},  tau)]=proj preG2.[( vis1{1},  tau)] /\
-    proj g1.[(!vis1{1},  tau)]=proj g2.[(!vis1{1},  tau)] /\
-    proj g1.[( vis1{1}, !tau)]=proj g2.[( vis1{1}, !tau)] /\
-    proj g1.[(!vis1{1}, !tau)]=proj g2.[(!vis1{1}, !tau)] /\
-    AdvGate.Adv.fc{1} = AdvGate.Adv.fc{2} /\
-    realChallenge{1} = !realChallenge{2} ).
-    rnd.
-
-    wp.
-    wp.
-admit.
-
-  if.
-
-    intros &1 &2 h.
-    rewrite (_:x1{1}=x1{2});[trivial|].
-    rewrite (_:AdvGate.Adv.fc{1}=AdvGate.Adv.fc{2});[trivial|].
-    simplify.
-    apply tr.
-
-    wp.
-    skip.
-    intros &1 &2 h.
-    split.
-    elim h; clear h; intros h h0;
-    elim h; clear h; intros h1 h;
-    elim h; clear h; intros h2 h;
-    elim h; clear h; intros h3 h;
-    elim h; clear h; intros h4 h;
-    elim h; clear h; intros h5 h;
-    elim h; clear h; intros h6 h;
-    elim h; clear h; intros h7 h;
-    elim h; clear h; intros h8 h;
-    elim h; clear h; intros h9 h;
-    elim h; clear h; intros h10 h;
-    elim h; clear h; intros h11 h;
-    elim h; clear h; intros h12 h13.
-    rewrite h1;
-    rewrite h2;
-    rewrite h3;
-    rewrite h4;
-    rewrite h5;
-    rewrite h6;
-    rewrite h7;
-    rewrite h8;
-    rewrite h9;
-    rewrite h10;
-    rewrite h11;
-    rewrite h12.
-    simplify.
-    admit.
-    intros hh L R hhh.
-    rewrite hhh.
-    clear hhh hh.
-    rewrite (_:realChallenge{1} = !realChallenge{2});[|clear h];trivial.
-
-    rnd.
-    skip.
-    intros &1 &2 h x y.
-    split.
-    trivial.
-    intros hh hhh.
-    split.
-    elim h; clear h; intros h h0;
-    elim h; clear h; intros h1 h;
-    elim h; clear h; intros h2 h;
-    elim h; clear h; intros h3 h;
-    elim h; clear h; intros h4 h;
-    elim h; clear h; intros h5 h;
-    elim h; clear h; intros h6 h;
-    elim h; clear h; intros h7 h;
-    elim h; clear h; intros h8 h;
-    elim h; clear h; intros h9 h;
-    elim h; clear h; intros h10 h;
-    elim h; clear h; intros h11 h;
-    elim h; clear h; intros h12 h13.
-    rewrite h1;
-    rewrite h2;
-    rewrite h3;
-    rewrite h4;
-    rewrite h5;
-    rewrite h6;
-    rewrite h7;
-    rewrite h8;
-    rewrite h9;
-    rewrite h10;
-    rewrite h11;
-    rewrite h12.
-    simplify.
-    admit.
-    intros hhhh L R hhhhh.
-    rewrite hhhhh.
-    clear hhhhh hhhh hhh hh.
-    rewrite (_:realChallenge{1} = !realChallenge{2});[|clear h]; trivial.
-
-    
-
-
-ssss
-  rcondf {1} 8;[admit|].
-  rcondf {1} 9;[admit|].
-  rcondt {1} 8;[admit|].   
-  rcondf {2} 8;[admit|].
-  rcondf {2} 8;[admit|].
-  rcondt {2} 8;[admit|].
-
-  call (answer{1}=answer{2}) (res{1}=res{2}). admit.
-    intros &m.
-    wp.
-rcondf {1} 1;[admit|].
-app 17 17 : (realChallenge{1}=realChallenge{2} /\ AdvGate.Adv.l{1}=1 /\ AdvGate.Adv.l{2}=2/\AdvGate.Adv.input{1}=AdvGate.Adv.input{2}).
-  admit.
-  app 2 3 : (realChallenge{1}=realChallenge{2} /\ AdvGate.Adv.l{1}=1 /\ AdvGate.Adv.l{2}=2/\AdvGate.Adv.g{1}=AdvGate.Adv.g{2}/\AdvGate.Adv.input{1}=AdvGate.Adv.input{2}).
-    rcondf {1} 1;[intros &m;skip;trivial|].
-    rcondt {1} 1;[intros &m;skip;trivial|].
-    rcondf {2} 1;[intros &m;skip;trivial|].
-    rcondf {2} 1;[intros &m;skip;trivial|].
-    rcondt {2} 1;[intros &m;skip;trivial|].
-    call (AdvGate.Adv.input{1}=AdvGate.Adv.input{2}) (AdvGate.Adv.g{1}=AdvGate.Adv.g{2}/\AdvGate.Adv.input{1}=AdvGate.Adv.input{2}).
-      fun.
-      admit.
-    intros L2 R2.
-    skip.
-    trivial.
-  rcondf {1} 1;[intros &m;skip;trivial|].
-  skip;intros _ _ _;split;trivial.
-save.
-*)
-
-lemma fakeEq :
-  forall (Adv <: Gate.Adv),
-    equiv [
-      Dkc.Game(Dkc.Dkc, AdvGate.Adv(Adv)).work ~ Dkc.Game(Dkc.Dkc, AdvGate.Adv(Adv)).work :
-      AdvGate.Adv.l{1}=2 ==> res{1} = res{2}
-    ]
-proof.
-  intros Adv.
-  fun.
-  inline {1} Dkc.Dkc.preInit.
-  inline {1} Dkc.Dkc.get_challenge.
-  inline {1} Dkc.Dkc.initialize.
-  rcondf {1} 7.
-    intros &m.
-    wp.
-    call (AdvGate.Adv.l = 2) (List.length res = 0).
-      fun.
-      app 4 : (AdvGate.Adv.l = 2).
-        wp.
-        call (true) (true). admit.
-        rnd.
-        skip.
-        trivial.
-      rcondf 1;[skip;trivial|].
-      rcondf 1;[skip;trivial|].
-      rcondt 1;[skip;trivial|].
-      call (true) (length res = 0). admit.
-    skip. trivial.
-    wp.
-    rnd.
-    skip.
-    trivial.
-swap {1} 1 6.
-swap {1} 9 -2.
-wp.
-(*Call magical function*)
-save.*)
-
-lemma fakeEq :
-  forall (Adv <: Gate.Adv),
-    equiv [
-      Dkc.Game(Dkc.Dkc, AdvGate.Adv(Adv)).work ~ RandBit.main :
-      (! Dkc.Dkc.b) /\ (AdvGate.Adv.l=1) ==> res{1} = res{2}
-    ]
-proof.
-intros Adv.
-fun.
-admit.
 save.
